theories/ftlr/Get.v
@@ -7,7 +7,7 @@ From cap_machine.rules Require Export rules_Get rules_base.
 From cap_machine Require Import stdpp_extra.
 
 Section fundamental.
-  Context {Σ:gFunctors} {memg:memG Σ} {regg:regG Σ} {sealsg: sealStoreG Σ}
+  Context {Σ:gFunctors} {ceriseg:ceriseG Σ} {sealsg: sealStoreG Σ}
           {nainv: logrel_na_invs Σ}
           `{MachineParameters}.
 
