theories/ftlr/Seal.v
@@ -6,7 +6,7 @@ From cap_machine.ftlr Require Import ftlr_base interp_weakening.
 From cap_machine.rules Require Import rules_base rules_Seal.
 
 Section fundamental.
-  Context {Σ:gFunctors} {memg:memG Σ} {regg:regG Σ} {sealsg: sealStoreG Σ}
+  Context {Σ:gFunctors} {ceriseg:ceriseG Σ} {sealsg: sealStoreG Σ}
           {nainv: logrel_na_invs Σ}
           `{MachineParameters}.
 
