theories/logrel.v
@@ -31,7 +31,7 @@ Class logrel_na_invs Σ :=
 
 (** interp : is a unary logical relation. *)
 Section logrel.
-  Context {Σ:gFunctors} {memg:memG Σ} {regg:regG Σ} {sealsg: sealStoreG Σ}
+  Context {Σ:gFunctors} {ceriseg:ceriseG Σ} {sealsg: sealStoreG Σ}
           {nainv: logrel_na_invs Σ}
           `{MachineParameters}.
 
