theories/rules/rules_EInit.v
@@ -5,8 +5,8 @@ From iris.algebra Require Import frac.
 From cap_machine Require Export rules_base.
 
 Section cap_lang_rules.
-  Context `{memG Σ, regG Σ}.
-  Context `{MachineParameters}.
+  Context `{ceriseg: ceriseG Σ}.
+  Context `{MP: MachineParameters}.
   Implicit Types P Q : iProp Σ.
   Implicit Types σ : ExecConf.
   Implicit Types c : cap_lang.expr.
