theories/rules/rules_EStoreId.v
@@ -5,8 +5,8 @@ From iris.algebra Require Import frac gmap.
 From cap_machine Require Export rules_base.
 
 Section cap_lang_rules.
-  Context `{memG Σ, regG Σ, enclavesG Σ}.
-  Context `{MachineParameters}.
+  Context `{ceriseg: ceriseG Σ}.
+  Context `{MP: MachineParameters}.
   Implicit Types P Q : iProp Σ.
   Implicit Types σ : ExecConf.
   Implicit Types c : cap_lang.expr.
@@ -24,58 +24,53 @@ Section cap_lang_rules.
   |EStoreId_spec_failure:
     EStoreId_spec FailedV.
 
-  Axiom has_lseal : LWord -> ENum -> Prop.
+  Axiom has_lseal : Z -> ENum -> Prop.
 
   (* TODO @Denis *)
-  Lemma wp_estoreid E pc_p pc_b pc_e pc_a pc_v lw rs1 rs2 rd seal p b e a v any x :
-    decodeInstrWL lw = EStoreId rs1 rs2 rd →
+  Lemma wp_estoreid E pc_p pc_b pc_e pc_a pc_v lw rd rs otype any :
+    decodeInstrWL lw = EStoreId rd rs →
     isCorrectLPC (LCap pc_p pc_b pc_e pc_a pc_v) →
-    writeAllowed p →
     {{{ PC ↦ᵣ LCap pc_p pc_b pc_e pc_a pc_v
         ∗ (pc_a, pc_v) ↦ₐ lw
-        ∗ rs1 ↦ᵣ seal
-        ∗ rs2 ↦ᵣ LCap p b e a v
+        ∗ rs ↦ᵣ LWInt otype
         ∗ rd ↦ᵣ any
-        ∗ (a, v) ↦ₐ x }}}
+    }}}
       Instr Executable @ E
     {{{ retv, RET retv;
         (pc_a, pc_v) ↦ₐ lw
         (* something with the pc increment *)
-        ∗ rs1 ↦ᵣ seal
-        ∗ rs2 ↦ᵣ LCap p b e a v
+        ∗ rs ↦ᵣ LWInt otype
         ∗ (
           ⌜ retv = NextIV ⌝
-          ∗ rd ↦ᵣ (LWInt 1)
           ∗ ∃ (id : EId), ∃ (enum : ENum),
-            (a, v) ↦ₐ (LWInt id)
-            ∗ (enclave_all enum id)
-            ∗ ⌜ has_lseal seal enum ⌝
+              rd ↦ᵣ (LWInt id)
+              ∗ (enclave_all enum id)
+            ∗ ⌜ has_lseal otype enum ⌝
         ) ∨ (
           ⌜ retv = FailedV ⌝
           ∗ rd ↦ᵣ any
-          ∗ (a, v) ↦ₐ x
         )
 
     }}}.
   Proof.
-    iIntros (Hinstr Hvpc Hwa φ) "(Hpc & Hpca & Hrs1 & Hrs2 & Hrd & Ha) Hφ".
+    iIntros (Hinstr Hvpc φ) "(Hpc & Hpca & Hrs & Hrd) Hφ".
     apply isCorrectLPC_isCorrectPC_iff in Hvpc; cbn in Hvpc.
     iApply wp_lift_atomic_head_step_no_fork; auto.
     iIntros (σ1 ns l1 l2 nt) "Hσ1 /=". destruct σ1; simpl.
-    iDestruct "Hσ1" as (lr lm vmap) "(Hr & Hm & %HLinv)"; simpl in HLinv.
-    iDestruct (@gen_heap_valid with "Hr Hpc") as %?.
-    iDestruct (@gen_heap_valid with "Hm Hpca") as %?.
-    iModIntro.
-    iSplitR. by iPureIntro; apply normal_always_head_reducible.
-    iIntros (e2 σ2 efs Hstep).
-    apply prim_step_exec_inv in Hstep as (-> & -> & (c & -> & Hstep)).
-    iNext; iIntros "_".
-    iSplitR; auto. eapply step_exec_inv in Hstep; eauto.
-    2: rewrite -/((lword_get_word (LCap pc_p pc_b pc_e pc_a pc_v)))
-    ; eapply state_corresponds_reg_get_word ; eauto.
-    2: eapply state_corresponds_mem_correct_PC ; eauto; cbn ; eauto.
-    cbn in Hstep; simplify_eq.
-    iModIntro.
+    (* iDestruct "Hσ1" as (lr lm vmap) "(Hr & Hm & %HLinv)"; simpl in HLinv. *)
+    (* iDestruct (@gen_heap_valid with "Hr Hpc") as %?. *)
+    (* iDestruct (@gen_heap_valid with "Hm Hpca") as %?. *)
+    (* iModIntro. *)
+    (* iSplitR. by iPureIntro; apply normal_always_head_reducible. *)
+    (* iIntros (e2 σ2 efs Hstep). *)
+    (* apply prim_step_exec_inv in Hstep as (-> & -> & (c & -> & Hstep)). *)
+    (* iNext; iIntros "_". *)
+    (* iSplitR; auto. eapply step_exec_inv in Hstep; eauto. *)
+    (* 2: rewrite -/((lword_get_word (LCap pc_p pc_b pc_e pc_a pc_v))) *)
+    (* ; eapply state_corresponds_reg_get_word ; eauto. *)
+    (* 2: eapply state_corresponds_mem_correct_PC ; eauto; cbn ; eauto. *)
+    (* cbn in Hstep; simplify_eq. *)
+    (* iModIntro. *)
     (* iSplitR "Hφ Hpc Hpca". last (iApply "Hφ" ; iFrame). *)
    (*  iExists lr, lm, vmap. *)
    (*  iFrame; auto. *)
